compiler/dsl/coq/ReflexEcho.v
@@ -1,0 +1,56 @@
+Require Import String.
+
+Require Import Reflex.
+Require Import ReflexBase.
+Require Import ReflexDenoted.
+Require Import ReflexVec.
+
+Definition NB_MSG : nat := 1.
+
+Definition PDV : payload_desc_vec NB_MSG :=
+  ( existT _ 1 (str_d, tt)
+  , tt
+  ).
+
+Definition HANDLERS : handler NB_MSG PDV :=
+  (fun m =>
+    match tag _ _ m as _tm return
+      @sdenote _ SDenoted_payload_desc (lkup_tag NB_MSG PDV _tm) -> _
+    with
+    | None => fun pl =>
+      let (s, _) := pl in
+         Send _ _ m
+           (CurChan _ _ _)
+           (MsgExpr _ _ m None (SLit _ _ m s, tt))
+      :: nil
+    | Some impossibru => fun _ =>
+      match impossibru with end
+    end (pay _ _ m)
+  )
+.
+
+Definition main := mk_main (Build_spec NB_MSG PDV HANDLERS).
+
+(*
+Axiom c : fd.
+
+Print kstate_run_prog. Check main.
+Eval compute in (msg NB_MSG PDV).
+Print msg.
+
+Require Import Ynot.
+
+Definition tr0 := [@nil (KAction NB_MSG PDV)]%inhabited.
+Definition ks0 := {|components := c :: nil; ktr := tr0|}.
+Definition m := (Build_msg NB_MSG PDV None (str_of_string "Hello", tt)).
+
+Eval compute in (
+  kstate_run_prog
+    NB_MSG
+    PDV
+    c
+    m
+    ks0
+    (HANDLERS m)
+).
+*)
